cedar-lean/Cedar/Thm/SymCC/Compiler/ExtHasAttr.lean
@@ -1,0 +1,673 @@
+/-
+ Copyright Cedar Contributors
+
+ Licensed under the Apache License, Version 2.0 (the "License");
+ you may not use this file except in compliance with the License.
+ You may obtain a copy of the License at
+
+      https://www.apache.org/licenses/LICENSE-2.0
+
+ Unless required by applicable law or agreed to in writing, software
+ distributed under the License is distributed on an "AS IS" BASIS,
+ WITHOUT WARRANTIES OR CONDITIONS OF ANY KIND, either express or implied.
+ See the License for the specific language governing permissions and
+ limitations under the License.
+-/
+
+import Cedar.Thm.SymCC.Compiler.Attr
+
+namespace Cedar.Thm
+
+open Batteries Data Spec SymCC Factory
+
+private theorem compileExtHasAttrRec_none_eq {ty : TermType} {a : Attr} {rest : List Attr} {εs : SymEntities} {t : Term}
+  (hwε : εs.WellFormed)
+  (hwt : (Term.none ty).WellFormed εs)
+  (hok : compileExtHasAttrRec (.none ty) (a :: rest) εs = .ok t) :
+  t = .none .bool
+:= by
+  cases rest with
+  | nil =>
+    simp only [compileExtHasAttrRec, bind, Except.bind] at hok
+    generalize hha : compileHasAttr (option.get (.none ty)) a εs = rha at hok
+    cases rha with
+    | error => simp only [reduceCtorEq] at hok
+    | ok t_ha =>
+    have hty_ha := (compileHasAttr_wf hwε (wf_option_get hwt (typeOf_term_none ty)).left hha).right
+    simp only [Except.ok.injEq] at hok
+    subst hok
+    exact pe_ifSome_none hty_ha
+  | cons b rest' =>
+    simp only [compileExtHasAttrRec, bind, Except.bind] at hok
+    generalize hha : compileHasAttr (option.get (.none ty)) a εs = rha at hok
+    cases rha with
+    | error => simp only [reduceCtorEq] at hok
+    | ok t_ha =>
+    have hty_ha := (compileHasAttr_wf hwε (wf_option_get hwt (typeOf_term_none ty)).left hha).right
+    have hifs_ha_eq := pe_ifSome_none (gty := ty) hty_ha
+    simp only [hifs_ha_eq] at hok
+    generalize hga : compileGetAttr (option.get (.none ty)) a εs = rga at hok
+    cases rga with
+    | error e =>
+      cases e <;> simp_all
+      simpa only [pure, Except.pure, Except.ok.injEq] using hok.symm
+    | ok t_ga =>
+    have ⟨_, ty_ga, hty_ga⟩ := compileGetAttr_wf hwε (wf_option_get hwt (typeOf_term_none ty)).left hga
+    have hifs_ga := pe_ifSome_none (gty := ty) hty_ga
+    simp only [hifs_ga] at hok
+    generalize hrest : compileExtHasAttrRec (.none ty_ga) (b :: rest') εs = rrest at hok
+    cases rrest with
+    | error => simp only [reduceCtorEq] at hok
+    | ok t_rest =>
+    have hwt_ga : (Term.none ty_ga).WellFormed εs := by
+      have h := typeOf_wf_term_is_wf (compileGetAttr_wf hwε (wf_option_get hwt (typeOf_term_none ty)).left hga).left
+      rw [hty_ga] at h; cases h; exact Term.WellFormed.none_wf (by assumption)
+    have hty_rest := (compileExtHasAttrRec_wf hwε hwt_ga ⟨_, typeOf_term_none _⟩ hrest).right
+    simp only [compileAnd, typeOf_term_none, bind, Except.bind, hty_rest, ↓reduceIte,
+      Except.ok.injEq] at hok
+    rw [← hok]
+    apply pe_ifSome_none
+    have hwog := wf_option_get
+      (Term.WellFormed.none_wf (εs := εs) TermType.WellFormed.bool_wf)
+      (typeOf_term_none .bool)
+    have hwt_rest :=
+      (compileExtHasAttrRec_wf hwε hwt_ga ⟨_, typeOf_term_none _⟩ hrest).left
+    have hwf_false : (⊙ Term.prim (TermPrim.bool false)).WellFormed εs :=
+      (wf_term_some (εs := εs) wf_bool typeOf_bool).left
+    have hty_ite := (wf_ite hwog.left hwt_rest hwf_false hwog.right
+      (by simp [someOf, typeOf_term_some, typeOf_bool, hty_rest])).right
+    simpa only [hty_rest] using hty_ite
+
+private theorem same_value_hasAttr {v : Value} {t' t_ha : Term} {a : Attr}
+  {es : Entities} {εs : SymEntities}
+  (heq : SameEntities es εs) (hwε : εs.WellFormed) (hwv : Value.WellFormed es v)
+  (hwt : t'.WellFormed εs)
+  (hha : compileHasAttr t' a εs = .ok t_ha)
+  (ih' : v ∼ t') :
+  (hasAttr v a es : Spec.Result Value) ∼ t_ha
+:= by
+  have hwφ₁ := Term.WellFormed.some_wf hwt
+  have hwo := wf_option_get hwφ₁ typeOf_term_some
+  have ih₁ := same_ok_some_iff.mpr ih'
+  have hwφ₂ := compileHasAttr_wf hwε hwo.left hha
+  replace ⟨t₃, rty, hattrs, ha⟩ := compileHasAttr_ok_implies hha
+  replace hattrs := compileAttrsOf_ok_implies hattrs
+  have hsame : (hasAttr v a es : Spec.Result Value) ∼ ifSome (Term.some t') t_ha := by
+    rcases hattrs with ⟨rty', htyₒ, ht₃⟩ | ⟨ety, fₐ, htyₒ, hf, ht₃⟩ <;> rw [ht₃] at ha
+    · exact compile_evaluate_hasAttr_record hwφ₁
+        (by rw [typeOf_term_some, htyₒ]) ⟨hwo.left, htyₒ⟩ hwφ₂ ha ih₁
+    · exact compile_evaluate_hasAttr_entity heq hwε hwv hwφ₁
+        (by rw [typeOf_term_some, htyₒ]) ⟨hwo.left, htyₒ⟩ hwφ₂ hf ha ih₁
+  rw [pe_ifSome_some hwφ₂.right] at hsame
+  exact hsame
+
+private theorem same_value_getAttr {v : Value} {t' t_ga : Term} {a : Attr}
+  {es : Entities} {εs : SymEntities}
+  (heq : SameEntities es εs) (hwε : εs.WellFormed) (hwv : Value.WellFormed es v)
+  (hwt : t'.WellFormed εs)
+  (hga : compileGetAttr t' a εs = .ok t_ga)
+  (ih' : v ∼ t') :
+  (getAttr v a es : Spec.Result Value) ∼ t_ga
+:= by
+  have hwφ₁ := Term.WellFormed.some_wf hwt
+  have hwo := wf_option_get hwφ₁ typeOf_term_some
+  have ih₁ := same_ok_some_iff.mpr ih'
+  have ⟨hwφ₂, tyₐ, htyₐ⟩ := compileGetAttr_wf hwε hwo.left hga
+  replace ⟨t₃, rty, hattrs, ha⟩ := compileGetAttr_ok_implies hga
+  replace hattrs := compileAttrsOf_ok_implies hattrs
+  have hsame : (getAttr v a es : Spec.Result Value) ∼ ifSome (Term.some t') t_ga := by
+    rcases hattrs with ⟨rty', htyₒ, ht₃⟩ | ⟨ety, fₐ, htyₒ, hf, ht₃⟩ <;> rw [ht₃] at ha
+    · exact compile_evaluate_getAttr_record hwφ₁
+        (by rw [typeOf_term_some, htyₒ]) ⟨hwo.left, htyₒ⟩ hwφ₂ htyₐ ha ih₁
+    · exact compile_evaluate_getAttr_entity heq hwε hwv hwφ₁
+        (by rw [typeOf_term_some, htyₒ]) ⟨hwo.left, htyₒ⟩ hwφ₂ htyₐ hf ha ih₁
+  rw [pe_ifSome_some htyₐ] at hsame
+  exact hsame
+
+private theorem getAttr_preserves_wf {v v_next : Value} {a : Attr} {es : Entities}
+  (hwe : es.WellFormed)
+  (hwv : Value.WellFormed es v)
+  (hga : getAttr v a es = .ok v_next) :
+  Value.WellFormed es v_next
+:= by
+  simp only [getAttr, attrsOf, Entities.attrs] at hga
+  cases v with
+  | prim p => cases p with
+    | entityUID uid =>
+      simp only [] at hga
+      generalize hfind : Map.findOrErr es uid Error.entityDoesNotExist = rfind at hga
+      cases rfind with
+      | error => simp only [Except.bind_err, reduceCtorEq] at hga
+      | ok d =>
+        simp only [Except.bind_ok] at hga
+        have hd : es.find? uid = .some d := by
+          simp only [Map.findOrErr_ok_iff_find?_some] at hfind; exact hfind
+        generalize hfa : Map.findOrErr d.attrs a Error.attrDoesNotExist = rfa at hga
+        cases rfa with
+        | error => simp only [reduceCtorEq] at hga
+        | ok v' =>
+          simp only [Except.ok.injEq] at hga; subst hga
+          have hv : d.attrs.find? a = .some v' := by
+            simp only [Map.findOrErr_ok_iff_find?_some] at hfa; exact hfa
+          have hwf_d := (hwe.right uid d hd).left
+          cases hwf_d; rename_i h₁ _; exact h₁ a v' hv
+    | _ => simp only [Except.bind_err, reduceCtorEq] at hga
+  | record avs =>
+    simp only [Except.bind_ok] at hga
+    generalize hfa : Map.findOrErr avs a Error.attrDoesNotExist = rfa at hga
+    cases rfa with
+    | error => simp only [reduceCtorEq] at hga
+    | ok v' =>
+      simp only [Except.ok.injEq] at hga; subst hga
+      have hv : avs.find? a = .some v' := by
+        simp only [Map.findOrErr_ok_iff_find?_some] at hfa; exact hfa
+      cases hwv; rename_i h₁ _; exact h₁ a v' hv
+  | set _ => simp only [Except.bind_err, reduceCtorEq] at hga
+  | ext _ => simp only [Except.bind_err, reduceCtorEq] at hga
+
+private theorem hasAttrs_loop_cons {v₁ v_next : Value} {a : Attr} {b : Attr} {rest : List Attr} {es : Entities}
+  (hha : hasAttr v₁ a es = .ok (.prim (.bool true)))
+  (hga : getAttr v₁ a es = .ok v_next) :
+  hasAttrs.loop v₁ (a :: b :: rest) es = hasAttrs.loop v_next (b :: rest) es
+:= by
+  cases v₁ with
+  | prim p => cases p with
+    | entityUID uid =>
+      simp only [hasAttr, attrsOf, Entities.attrsOrEmpty, Map.contains, Except.bind_ok,
+        Except.ok.injEq] at hha
+      simp only [getAttr, attrsOf, Entities.attrs] at hga
+      generalize hfind : Map.findOrErr es uid Error.entityDoesNotExist = rfind at hga
+      cases rfind with
+      | error => simp only [Except.bind_err, reduceCtorEq] at hga
+      | ok d =>
+        simp only [Except.bind_ok] at hga
+        have hd : es.find? uid = .some d := by
+          simp only [Map.findOrErr_ok_iff_find?_some] at hfind; exact hfind
+        have hfa : d.attrs.find? a = .some v_next := by
+          simp only [Map.findOrErr_ok_iff_find?_some] at hga; exact hga
+        simp only [hasAttrs.loop, attrsOf, Entities.attrsOrEmpty, hd, hfa]
+    | _ => simp only [hasAttr, attrsOf, Except.bind_err, reduceCtorEq] at hha
+  | record avs =>
+    simp only [getAttr, attrsOf, Except.bind_ok] at hga
+    have hfa : avs.find? a = .some v_next := by
+      simp only [Map.findOrErr_ok_iff_find?_some] at hga; exact hga
+    simp only [hasAttrs.loop, attrsOf, hfa]
+  | set _ => simp only [hasAttr, attrsOf, Except.bind_err, reduceCtorEq] at hha
+  | ext _ => simp only [hasAttr, attrsOf, Except.bind_err, reduceCtorEq] at hha
+
+
+private theorem hasAttr_returns_bool {v₁ : Value} {a : Attr} {es : Entities} {v : Value}
+  (hha : hasAttr v₁ a es = .ok v) : ∃ b, v = .prim (.bool b) := by
+  simp only [hasAttr, attrsOf] at hha
+  cases v₁ with
+  | prim p => cases p with
+    | entityUID _ => simp only [Except.bind_ok, Except.ok.injEq] at hha; subst hha; exact ⟨_, rfl⟩
+    | _ => simp at hha
+  | record _ => simp only [Except.bind_ok, Except.ok.injEq] at hha; subst hha; exact ⟨_, rfl⟩
+  | set _ => simp at hha
+  | ext _ => simp at hha
+
+private theorem hasAttrs_loop_singleton_eq_hasAttr {v₁ : Value} {a : Attr} {es : Entities} :
+    hasAttrs.loop v₁ [a] es = hasAttr v₁ a es := by
+  simp only [hasAttrs.loop, hasAttr, attrsOf]
+  cases v₁ with
+  | prim p => cases p with
+    | entityUID uid => simp [Map.contains, Option.isSome]; cases (es.attrsOrEmpty uid).find? a <;> simp
+    | _ => simp
+  | record avs => simp [Map.contains, Option.isSome]; cases avs.find? a <;> simp
+  | set _ => simp
+  | ext _ => simp
+
+private theorem hasAttr_true_implies_getAttr_ok {v₁ : Value} {a : Attr} {es : Entities} {e : Spec.Error}
+    (hha : hasAttr v₁ a es = .ok (.prim (.bool true)))
+    (hga : getAttr v₁ a es = .error e) : False := by
+  simp only [hasAttr, getAttr, attrsOf, Entities.attrs, Entities.attrsOrEmpty, Map.contains] at hha hga
+  cases v₁ with
+  | prim p => cases p with
+    | entityUID uid =>
+      simp only [Except.bind_ok, Except.ok.injEq] at hha
+      simp only [] at hga
+      generalize hfind : Map.findOrErr es uid Error.entityDoesNotExist = rf at hga
+      cases rf with
+      | error =>
+        simp only [Map.findOrErr] at hfind
+        split at hfind
+        · simp only [reduceCtorEq] at hfind
+        · rename_i hfn
+          have hfn' : es.find? uid = .none := by
+            cases h : es.find? uid with
+            | none => rfl
+            | some d => exact (hfn d h).elim
+          simp [hfn', Option.isSome] at hha
+      | ok d =>
+        simp only [Except.bind_ok] at hga
+        have hd := Map.findOrErr_ok_iff_find?_some.mp hfind
+        simp only [hd, Option.isSome] at hha
+        simp only [Map.findOrErr] at hga
+        split at hga
+        · simp only [reduceCtorEq] at hga
+        · rename_i hn
+          cases hf : d.attrs.find? a with
+          | some v => exact hn v hf
+          | none => simp [hf] at hha
+    | _ => simp only [Except.bind_err, reduceCtorEq] at hha
+  | record avs =>
+    simp only [Except.bind_ok, Except.ok.injEq] at hha
+    simp only [Except.bind_ok, Map.findOrErr] at hga
+    split at hga
+    · simp only [reduceCtorEq] at hga
+    · rename_i hn
+      cases hf : avs.find? a with
+      | some v => exact hn v hf
+      | none => simp [hf, Option.isSome] at hha
+  | set _ => simp only [Except.bind_err, reduceCtorEq] at hha
+  | ext _ => simp only [Except.bind_err, reduceCtorEq] at hha
+
+private theorem hasAttrs_loop_false {v₁ : Value} {a : Attr} {rest : List Attr} {es : Entities}
+  (hha : hasAttr v₁ a es = .ok (.prim (.bool false))) :
+  hasAttrs.loop v₁ (a :: rest) es = .ok (.prim (.bool false)) := by
+  simp only [hasAttr] at hha
+  generalize hattr : attrsOf v₁ (fun uid => .ok (Entities.attrsOrEmpty es uid)) = rattr at hha
+  cases rattr with
+  | error => simp at hha
+  | ok r =>
+    simp only [Except.bind_ok, Except.ok.injEq, Value.prim.injEq, Prim.bool.injEq] at hha
+    have hfind : r.find? a = .none := by
+      simp only [Map.contains, Option.isSome_eq_false_iff] at hha
+      exact Option.not_isSome_iff_eq_none.mp (by simp [hha])
+    simp only [hasAttrs.loop, hattr, hfind]
+
+
+private theorem compileHasAttr_eq_false_of_compileGetAttr_error
+  {t t_ha : Term} {a : Attr} {εs : SymEntities} {e : SymCC.Error}
+  (hha : compileHasAttr t a εs = .ok t_ha)
+  (hga : compileGetAttr t a εs = .error e) :
+  t_ha = (⊙ false)
+:= by
+  obtain ⟨t₂, rty, hattrs, hrecord⟩ := compileHasAttr_ok_implies hha
+  simp only [RecordHasAttr] at hrecord
+  simp only [compileGetAttr, hattrs, Except.bind_ok, hrecord.left] at hga
+  split at hga <;> simp_all [someOf]
+
+private theorem compile_evaluate_extHasAttr_loop
+  {v₁ : Value} {t₁' : Term} {a : Attr} {l : List Attr}
+  {es : Entities} {εs : SymEntities} {t : Term}
+  (heq : SameEntities es εs)
+  (hwε : εs.WellFormed)
+  (hwe : es.WellFormed)
+  (hwv : Value.WellFormed es v₁)
+  (hwt : t₁'.WellFormed εs)
+  (hok : compileExtHasAttrRec (.some t₁') (a :: l) εs = .ok t)
+  (ih' : v₁ ∼ t₁') :
+  hasAttrs.loop v₁ (a :: l) es ∼ t
+:= by
+  induction l generalizing a v₁ t₁' t with
+  | nil =>
+    simp only [compileExtHasAttrRec, bind, Except.bind] at hok
+    generalize h₁ : compileHasAttr (option.get (Term.some t₁')) a εs = rha at hok
+    cases rha with
+    | error => simp only [reduceCtorEq] at hok
+    | ok t_ha =>
+      simp only [pe_option_get_some] at h₁
+      have h₂ := (compileHasAttr_wf hwε (wf_option_get (Term.WellFormed.some_wf hwt) typeOf_term_some).left h₁).right
+      simp only [pe_ifSome_some h₂, Except.ok.injEq] at hok
+      subst hok
+      rw [hasAttrs_loop_singleton_eq_hasAttr]
+      exact same_value_hasAttr heq hwε hwv hwt h₁ ih'
+  | cons b rest ih =>
+    simp only [compileExtHasAttrRec, bind, Except.bind] at hok
+    generalize h₁ : compileHasAttr (option.get (Term.some t₁')) a εs = rha at hok
+    cases rha with
+    | error => simp only [reduceCtorEq] at hok
+    | ok t_ha =>
+    simp only [pe_option_get_some] at h₁
+    have h₃ := (compileHasAttr_wf hwε (wf_option_get (Term.WellFormed.some_wf hwt) typeOf_term_some).left h₁).right
+    have h₄ := same_value_hasAttr heq hwε hwv hwt h₁ ih'
+    generalize h₅ : hasAttr v₁ a es = rha_v at h₄
+    cases rha_v with
+    | error e =>
+      exfalso
+      obtain ⟨t_attrs, rty, hattrs, _⟩ := compileHasAttr_ok_implies h₁
+      have hattrs_impl := compileAttrsOf_ok_implies hattrs
+      have hv_same : t₁'.value? = .some v₁ := same_implies_same_value ih'
+      simp only [hasAttr, attrsOf] at h₅
+      rcases hattrs_impl with ⟨_, hty_rec, _⟩ | ⟨ety, _, hty_ent, _, _⟩
+      · have hlit := same_value_implies_lit ih'
+        have ⟨rt, hrt⟩ := wfl_of_type_record_is_record ⟨hwt, hlit⟩ hty_rec
+        subst hrt
+        have ⟨rv, _, _⟩ := same_record_term_implies (same_implies_same_value ih')
+        subst_vars
+        simp at h₅
+      · have hlit := same_value_implies_lit ih'
+        have ⟨uid, huid, _⟩ := wfl_of_type_entity_is_entity ⟨hwt, hlit⟩ hty_ent
+        subst huid
+        simp only [Same.same, SameValues, Term.value?, TermPrim.value?, Option.some.injEq] at ih'
+        subst ih'
+        simp at h₅
+    | ok v_ha =>
+      have ⟨b_val, hb_val⟩ := hasAttr_returns_bool h₅
+      subst hb_val
+      have htha_eq := same_ok_bool_implies h₄; subst htha_eq
+      cases b_val with
+      | false =>
+        simp only [pe_ifSome_some h₃, pure, Except.pure, Except.ok.injEq] at hok
+        subst t
+        rw [hasAttrs_loop_false h₅]
+        exact h₄
+      | true =>
+        have hok' := hok
+        revert hok'
+        simp only [pe_option_get_some, pe_ifSome_some h₃]
+        intro hok'
+        generalize hga : compileGetAttr t₁' a εs = rga at hok'
+        cases rga with
+        | error e =>
+          have ht_ha := compileHasAttr_eq_false_of_compileGetAttr_error h₁ hga
+          simp [someOf] at ht_ha
+        | ok t_ga =>
+        simp only [] at hok'
+        have ⟨hwt_ga, _, hty_ga⟩ := compileGetAttr_wf hwε (wf_option_get (Term.WellFormed.some_wf hwt) typeOf_term_some).left hga
+        have hsame_ga := same_value_getAttr heq hwε hwv hwt hga ih'
+        generalize hga_v : getAttr v₁ a es = rga_v at hsame_ga
+        cases rga_v with
+        | error e_ga =>
+          exfalso; exact hasAttr_true_implies_getAttr_ok h₅ hga_v
+        | ok v_next =>
+          have ⟨t_ga', ht_ga_eq, hv_ga⟩ := same_ok_implies hsame_ga
+          subst ht_ga_eq
+          simp only [pe_ifSome_some hty_ga] at hok'
+          generalize hrest : compileExtHasAttrRec (Term.some t_ga') (b :: rest) εs = r_rest at hok'
+          cases r_rest with
+          | ok t_rest =>
+            have hty_some_ga : ∃ ty, (Term.some t_ga').typeOf = .option ty :=
+              ⟨_, typeOf_term_some⟩
+            have hty_rest := (compileExtHasAttrRec_wf hwε (Term.WellFormed.some_wf (wf_term_some_implies hwt_ga)) hty_some_ga hrest).right
+            simp only [compileAnd, typeOf_term_some, typeOf_bool, bind, Except.bind, hty_rest,
+              ↓reduceIte, pe_option_get_some, pe_ite_true, pe_ifSome_some hty_rest,
+              Except.ok.injEq] at hok'
+            subst hok'
+            rw [hasAttrs_loop_cons h₅ hga_v]
+            have hwv_next := getAttr_preserves_wf hwe hwv hga_v
+            exact ih hwv_next (wf_term_some_implies hwt_ga) hrest hv_ga
+          | error => simp only [] at hok'; contradiction
+
+theorem compile_evaluate_extHasAttr {x₁ : Expr} {a : Attr} {l : List Attr} {env : Env} {εnv : SymEnv} {t : Term}
+  (heq : env ∼ εnv)
+  (hwe : env.WellFormedFor (.extHasAttr x₁ a l))
+  (hwε : εnv.WellFormedFor (.extHasAttr x₁ a l))
+  (hok : compile (.extHasAttr x₁ a l) εnv = .ok t)
+  (ih  : CompileEvaluate x₁) :
+  evaluate (.extHasAttr x₁ a l) env.request env.entities ∼ t
+:= by
+  unfold CompileEvaluate at ih
+  rw [compile.eq_def] at hok
+  simp only at hok
+  simp_do_let (compile x₁ εnv) at hok
+  rename_i t₁ hok₁
+  rw [compileExtHasAttr_eq_compileExtHasAttrRec] at hok
+  replace hwe := wf_env_for_extHasAttr_implies hwe
+  have hwφ₁ := wf_εnv_for_extHasAttr_implies hwε
+  have ⟨hwt₁, ty₁, hty₁⟩ := compile_wf hwφ₁ hok₁
+  have hce := compileExtHasAttrRec_wf hwε.left.right hwt₁ ⟨ty₁, hty₁⟩ hok
+  replace ih := ih heq hwe hwφ₁ hok₁
+  unfold evaluate
+  simp_do_let (evaluate x₁ env.request env.entities)
+  case error e he =>
+    rw [he] at ih
+    have ⟨hne, ty', ht₁⟩ := same_error_implies ih
+    subst ht₁
+    have ht : t = .none .bool := compileExtHasAttrRec_none_eq hwε.left.right hwt₁ hok
+    subst ht
+    exact same_error_implied_by hne
+  case ok v₁ hv₁ =>
+    rw [hv₁] at ih
+    have ⟨t₁', ht₁, ih'⟩ := same_ok_implies ih
+    subst ht₁
+    exact compile_evaluate_extHasAttr_loop heq.right hwε.left.right hwe.left.right
+      (evaluate_wf hwe hv₁) (wf_term_some_implies hwt₁) hok ih'
+
+private theorem compileAnd_interpret {t₁ t₂ t : Term} {εnv : SymEnv} {I : Interpretation}
+  (hI : I.WellFormed εnv.entities)
+  (hw₁ : t₁.WellFormed εnv.entities) (hty₁ : t₁.typeOf = .option .bool)
+  (hw₂ : t₂.WellFormed εnv.entities) (hty₂ : t₂.typeOf = .option .bool)
+  (hok : compileAnd t₁ (.ok t₂) = .ok t) :
+  compileAnd (t₁.interpret I) (.ok (t₂.interpret I)) = .ok (t.interpret I)
+:= by
+  have h₁ := wf_option_get hw₁ hty₁
+  have h₂ := @wf_ite εnv.entities (option.get t₁) t₂ (Term.some (Term.prim (TermPrim.bool false)))
+    h₁.left hw₂ (Term.WellFormed.some_wf wf_bool)
+    h₁.right (by simp only [Term.typeOf, typeOf_bool, hty₂])
+  have h₃ : (t₁.interpret I).typeOf = .option .bool := by
+    rw [(interpret_term_wf hI hw₁).right]; exact hty₁
+  have h₄ : (t₂.interpret I).typeOf = .option .bool := by
+    rw [(interpret_term_wf hI hw₂).right]; exact hty₂
+  by_cases h₅ : t₁ = Term.some (Term.prim (TermPrim.bool false))
+  case pos =>
+    subst h₅
+    simp only [compileAnd, Except.ok.injEq] at hok
+    subst hok
+    simp only [compileAnd, interpret_term_some, interpret_term_prim]
+  case neg =>
+    have hok' : compileAnd t₁ (.ok t₂) = .ok t := hok
+    simp only [compileAnd] at hok
+    split at hok
+    case h_1 heq => contradiction
+    case h_2 =>
+      simp only [Except.bind_ok, hty₂, ↓reduceIte, Except.ok.injEq] at hok; subst hok
+      simp only [someOf, interpret_ifSome hI hw₁ h₂.left,
+        interpret_ite hI h₁.left hw₂ (wf_term_some wf_bool rfl).left
+          h₁.right (by simp only [typeOf_term_some, typeOf_bool, hty₂]),
+        interpret_option_get I hw₁ hty₁,
+        interpret_term_some, interpret_term_prim]
+      simp only [compileAnd]
+      split
+      case h_1 heq_i =>
+        simp only [Except.ok.injEq, heq_i]
+        simp only [pe_option_get'_some, pe_ite_false, pe_ifSome_some typeOf_term_some]
+      case h_2 _ =>
+        simp only [someOf, h₄, ↓reduceIte, Except.bind_ok, Except.ok.injEq, ExceptT.stM_eq]
+        have hwfl := interpret_term_wfl hI hw₁
+        rw [hty₁] at hwfl
+        have h₆ := interpret_entities_same_domain εnv.entities I
+        have h₇ := wf_term_same_domain h₆ (interpret_term_wf hI hw₁).left
+        have h₈ := wf_term_same_domain h₆ (interpret_term_wf hI hw₂).left
+        have h₉ := wf_option_get h₇ h₃
+        have h₁₀ := wf_option_get' hI (interpret_term_wf hI hw₁).left h₃
+        have h₁₁ := wf_term_same_domain h₆ h₁₀.left
+        have h₁₂ : (Term.some (.prim (.bool false))).WellFormed (εnv.entities.interpret I) :=
+          Term.WellFormed.some_wf (wf_bool (εs := εnv.entities.interpret I))
+        have h₁₃ := (wf_ite h₉.left h₈ h₁₂ h₉.right
+          (by simp only [typeOf_term_some, typeOf_bool, h₄])).right
+        have h₁₄ := (wf_ite h₁₁ h₈ h₁₂ h₁₀.right
+          (by simp only [typeOf_term_some, typeOf_bool, h₄])).right
+        rw [h₄] at h₁₃ h₁₄
+        exact pe_ifSome_get_eq_get' I
+          (fun x => Factory.ite x (t₂.interpret I) (.some (.prim (.bool false))))
+          hwfl.left hwfl.right h₁₃ h₁₄
+      case h_3 hty_i =>
+        exfalso; simp only [h₃, imp_false, not_true_eq_false] at hty_i
+    case h_3 hty =>
+      rw [hty₁] at hty; simp at hty
+
+private theorem compileExtHasAttrRec_interpret {t₁ : Term} {attrs : List Attr} {εnv : SymEnv} {I : Interpretation} {t : Term}
+  (hI : I.WellFormed εnv.entities)
+  (hwε : εnv.entities.WellFormed)
+  (hw₁ : t₁.WellFormed εnv.entities) (hty₁ : ∃ ty, t₁.typeOf = .option ty)
+  (hok : compileExtHasAttrRec t₁ attrs εnv.entities = .ok t) :
+  compileExtHasAttrRec (t₁.interpret I) attrs (εnv.entities.interpret I) = .ok (t.interpret I)
+:= by
+  induction attrs generalizing t₁ t with
+  | nil =>
+    simp only [compileExtHasAttrRec, pure, Except.pure, Except.ok.injEq] at hok ⊢
+    subst hok
+    simp [interpret_term_some, interpret_term_prim]
+  | cons a rest ih =>
+    cases rest with
+    | nil =>
+      simp only [compileExtHasAttrRec, bind, Except.bind] at hok ⊢
+      generalize h₁ : compileHasAttr (option.get t₁) a εnv.entities = rha at hok
+      cases rha with
+      | error => simp only [reduceCtorEq] at hok
+      | ok t_ha =>
+        simp only [Except.ok.injEq] at hok; subst hok
+        have h₂ := wf_option_get hw₁ hty₁.choose_spec
+        have h₃ := interpret_compileHasAttr hwε hI h₂.left h₁
+        have h₄ := interpret_εntities_wf hwε hI
+        have h₅ := (compileHasAttr_wf hwε h₂.left h₁).left
+        have h₆ := (compileHasAttr_wf hwε h₂.left h₁).right
+        simp_do_let (compileHasAttr (option.get (Term.interpret I t₁)) a (SymEntities.interpret I εnv.entities)) <;>
+        rename_i h₇
+        case error =>
+          have ⟨_, hok'⟩ := compileHasAttr_interpret_ok hI hwε hw₁ hty₁.choose_spec h₃
+          simp only [hok', reduceCtorEq] at h₇
+        case ok t₄ =>
+          simp only [interpret_ifSome hI hw₁ h₅, Except.ok.injEq]
+          rw [interpret_option_get I hw₁ hty₁.choose_spec] at h₃
+          have hwφ₂ := interpret_term_wfl hI hw₁; rw [hty₁.choose_spec] at hwφ₂
+          have h₈ : t₄.typeOf = .option .bool := by
+            have h₉ := wf_option_get hwφ₂.left.left hwφ₂.right
+            have h₁₀ := wf_term_same_domain (interpret_entities_same_domain εnv.entities I) h₉.left
+            exact (compileHasAttr_wf h₄ h₁₀ h₇).right
+          rw [← (interpret_term_wf hI h₅).right] at h₆
+          exact pe_ifSome_ok_get_eq_get' I (compileHasAttr · a (SymEntities.interpret I εnv.entities))
+            hwφ₂ h₆ h₈ h₃ h₇
+    | cons b rest' =>
+      simp only [compileExtHasAttrRec, bind, Except.bind] at hok ⊢
+      generalize h₁ : compileHasAttr (option.get t₁) a εnv.entities = rha at hok
+      cases rha with
+      | error => simp only [reduceCtorEq] at hok
+      | ok h₃ =>
+        generalize h₂ : compileGetAttr (option.get t₁) a εnv.entities = rga at hok
+        cases rga with
+        | error e =>
+          have h₄ := compileHasAttr_eq_false_of_compileGetAttr_error h₁ h₂
+          subst h₃
+          have h₅ := wf_option_get hw₁ hty₁.choose_spec
+          have h₆ := interpret_compileHasAttr hwε hI h₅.left h₁
+          have h₇ := interpret_εntities_wf hwε hI
+          have ⟨h₈, h₉, h₁₀⟩ := interpret_option_get_aux hI hw₁ hty₁.choose_spec
+          have h₁₁ := interpret_compileGetAttr_error_of_compileHasAttr_false hwε hI h₅.left h₁ h₂
+          simp only [interpret_someOf, interpret_term_prim] at h₆
+          have h₁₂ := compileHasAttr_false_of_getAttr_error_typeOf_eq h₇ h₈ h₉ h₁₀ h₆ h₁₁
+          have h₁₃ := compileGetAttr_noSuchAttribute_of_error_typeOf_eq h₇ h₈ h₉ h₁₀ h₆ h₁₁
+          have h₁₄ := (compileHasAttr_wf hwε h₅.left h₁).left
+          simp only [] at hok
+          split at hok
+          case h_1 heq =>
+            simp only [pure, Except.pure, Except.ok.injEq] at hok
+            subst t
+            simp only [h₁₂]
+            have h₁₅ := congrArg (Term.interpret I) heq
+            rw [interpret_ifSome hI hw₁ h₁₄] at h₁₅
+            simp only [interpret_someOf, interpret_term_prim] at h₁₅
+            simp only [someOf] at heq h₁₅ ⊢
+            simp only [interpret_term_some, interpret_term_prim] at h₁₅
+            rw [h₁₅, heq]
+            simp only [interpret_term_some, interpret_term_prim, pure, Except.pure]
+          case h_2 =>
+            cases e <;> simp_all
+            simp only [pure, Except.pure, Except.ok.injEq] at hok
+            subst t
+            rw [interpret_ifSome hI hw₁ h₁₄]
+            simp only [interpret_someOf, interpret_term_prim]
+            split
+            all_goals simp only [someOf, pure, Except.pure]
+        | ok t_ga =>
+          have h₅ := wf_option_get hw₁ hty₁.choose_spec
+          have h₆ := interpret_εntities_wf hwε hI
+          have h₇ := (compileHasAttr_wf hwε h₅.left h₁).left
+          have h₈ := (compileHasAttr_wf hwε h₅.left h₁).right
+          have ⟨h₉, tyₐ, h₁₀⟩ := compileGetAttr_wf hwε h₅.left h₂
+          have h₁₁ := interpret_compileHasAttr hwε hI h₅.left h₁
+          have h₁₂ := interpret_compileGetAttr hwε hI h₅.left h₂
+          simp_do_let (compileHasAttr (option.get (Term.interpret I t₁)) a (SymEntities.interpret I εnv.entities)) <;>
+          rename_i h₁₃
+          case error =>
+            have ⟨_, h₁₄⟩ := compileHasAttr_interpret_ok hI hwε hw₁ hty₁.choose_spec h₁₁
+            rw [h₁₄] at h₁₃
+            simp at h₁₃
+          case ok t_ha' =>
+          have ⟨t_ga', h₁₄⟩ := compileGetAttr_interpret_ok hI hwε hw₁ hty₁.choose_spec h₁₂
+          simp only [h₁₄]
+          simp only [] at hok
+          have h₁₅ := (wf_ifSome_option hw₁ h₉ h₁₀).left
+          have h₁₆ : ∃ ty, (ifSome t₁ t_ga).typeOf = .option ty :=
+            ⟨_, (wf_ifSome_option hw₁ h₉ h₁₀).right⟩
+          have h₁₇ := interpret_term_wfl hI hw₁
+          rw [hty₁.choose_spec] at h₁₇
+          have h₁₈ := interpret_entities_same_domain εnv.entities I
+          have h₁₉ := wf_option_get h₁₇.left.left h₁₇.right
+          have h₂₀ := wf_term_same_domain h₁₈ h₁₉.left
+          have h₂₁ := wf_term_same_domain h₁₈ (interpret_term_wf hI h₅.left).left
+          have h₂₂ : (t_ga.interpret I).typeOf = .option tyₐ :=
+            (interpret_term_wf hI h₉).right.trans h₁₀
+          have h₂₃ : t_ga'.typeOf = .option tyₐ := by
+            have h₂₄ := compileGetAttr_ok_typeOf_eq h₆ h₂₁ h₂₀
+              (by exact (interpret_term_wf hI h₅.left).right.trans (h₅.right.trans h₁₉.right.symm)) h₁₂ h₁₄
+            exact h₂₄.trans h₂₂
+          rw [interpret_option_get I hw₁ hty₁.choose_spec] at h₁₁ h₁₂
+          have h₂₄ := pe_ifSome_ok_get_eq_get' I
+            (compileGetAttr · a (SymEntities.interpret I εnv.entities))
+            h₁₇ h₂₂ h₂₃ h₁₂ h₁₄
+          have h₂₅ : (h₃.interpret I).typeOf = .option .bool :=
+            (interpret_term_wf hI h₇).right.trans h₈
+          have h₂₆ : t_ha'.typeOf = .option .bool :=
+            (compileHasAttr_wf h₆ h₂₀ h₁₃).right
+          have h₂₇ := pe_ifSome_ok_get_eq_get' I
+            (compileHasAttr · a (SymEntities.interpret I εnv.entities))
+            h₁₇ h₂₅ h₂₆ h₁₁ h₁₃
+          generalize h₂₈ : compileExtHasAttrRec (ifSome t₁ t_ga) (b :: rest') εnv.entities = rrest at hok
+          cases rrest with
+          | ok t_rest =>
+            have h₂₉ := ih h₁₅ h₁₆ h₂₈
+            rw [interpret_ifSome hI hw₁ h₉] at h₂₉
+            rw [h₂₄, h₂₉, h₂₇]
+            have h₃₀ := (wf_ifSome_option hw₁ h₇ h₈).left
+            have h₃₁ := (wf_ifSome_option hw₁ h₇ h₈).right
+            have h₃₂ := (compileExtHasAttrRec_wf hwε h₁₅ h₁₆ h₂₈).left
+            have h₃₃ := (compileExtHasAttrRec_wf hwε h₁₅ h₁₆ h₂₈).right
+            rw [← interpret_ifSome hI hw₁ h₇]
+            split at hok
+            case h_1 h₃₄ =>
+              simp only [pure, Except.pure, Except.ok.injEq] at hok
+              subst t
+              rw [h₃₄]
+              simp only [interpret_term_some, interpret_term_prim, pure, Except.pure]
+            case h_2 =>
+              have h₃₄ := compileAnd_interpret hI h₃₀ h₃₁ h₃₂ h₃₃ hok
+              split
+              case h_1 h₃₅ =>
+                rw [h₃₅] at h₃₄ ⊢
+                simpa only [pure, Except.pure, compileAnd] using h₃₄
+              case h_2 => exact h₃₄
+          | error =>
+            simp only [] at hok
+            split at hok
+            case h_1 h₂₉ =>
+              simp only [pure, Except.pure, Except.ok.injEq] at hok
+              subst t
+              rw [h₂₇, ← interpret_ifSome hI hw₁ h₇, h₂₉]
+              simp only [interpret_term_some, interpret_term_prim, pure, Except.pure]
+            case h_2 => simp only [reduceCtorEq] at hok
+
+theorem compile_interpret_extHasAttr {x₁ : Expr} {a : Attr} {l : List Attr} {εnv : SymEnv} {I : Interpretation} {t : Term}
+  (hI  : I.WellFormed εnv.entities)
+  (hwε : εnv.WellFormedFor (.extHasAttr x₁ a l))
+  (hok : compile (.extHasAttr x₁ a l) εnv = .ok t)
+  (ih  : CompileInterpret x₁) :
+  compile (.extHasAttr x₁ a l) (εnv.interpret I) = .ok (t.interpret I)
+:= by
+  have hwφ₁ := wf_εnv_for_extHasAttr_implies hwε
+  rw [compile.eq_def] at hok
+  simp only at hok
+  simp_do_let (compile x₁ εnv) at hok
+  rename_i t₁ hok₁
+  rw [compileExtHasAttr_eq_compileExtHasAttrRec] at hok
+  have ⟨hwt₁, ty₁, hty₁⟩ := compile_wf hwφ₁ hok₁
+  have ih₁ := ih hI hwφ₁ hok₁
+  simp only [compile, ih₁, Except.bind_ok]
+  simp only [SymEnv.interpret]
+  rw [compileExtHasAttr_eq_compileExtHasAttrRec]
+  exact compileExtHasAttrRec_interpret hI hwε.left.right hwt₁ ⟨ty₁, hty₁⟩ hok
+
+end Cedar.Thm
